WIP

src/coq/Handlers/Global.v
@@ -7,9 +7,13 @@ From ExtLib Require Import
 
 From ITree Require Import
      ITree
-     Events.State.
+     Events.State
+     Eq.Eq
+     Events.StateFacts
+     InterpFacts.
 
 From Vellvm Require Import
+     Util
      LLVMAst
      AstLib
      MemoryAddress
@@ -46,17 +50,42 @@ Section Globals.
   Open Scope monad_scope.
   Section PARAMS.
     Variable (E F G : Type -> Type).
-    Definition E_trigger {M} : forall R, E R -> (stateT M (itree (E +' F +' G)) R) :=
+    Context `{FailureE -< E +' F +' G}.
+    Notation Effin := (E +' F +' (GlobalE k v) +' G).
+    Notation Effout := (E +' F +' G).
+
+    Definition E_trigger {M} : forall R, E R -> (stateT M (itree Effout) R) :=
       fun R e m => r <- trigger e ;; ret (m, r).
 
-    Definition F_trigger {M} : forall R, F R -> (stateT M (itree (E +' F +' G)) R) :=
+    Definition F_trigger {M} : forall R, F R -> (stateT M (itree Effout) R) :=
       fun R e m => r <- trigger e ;; ret (m, r).
 
-    Definition G_trigger {M} : forall R , G R -> (stateT M (itree (E +' F +' G)) R) :=
+    Definition G_trigger {M} : forall R , G R -> (stateT M (itree Effout) R) :=
       fun R e m => r <- trigger e ;; ret (m, r).
 
-    Definition interp_global `{FailureE -< E +' F +' G} : itree (E +' F +' (GlobalE k v) +' G) ~> stateT map (itree (E +' F +' G)) :=
+    Definition interp_global  : itree Effin ~> stateT map (itree Effout) :=
       interp_state (case_ E_trigger (case_ F_trigger (case_ handle_global G_trigger))).
+
+    Lemma interp_global_bind :
+      forall (R S : Type) (t : itree Effin R) (k : R -> itree Effin S) s,
+        runState (interp_global (ITree.bind t k)) s ≅
+         ITree.bind (runState (interp_global t) s) (fun '(s',r) => runState (interp_global (k r)) s').
+    Proof.
+      intros.
+      unfold interp_global.
+      setoid_rewrite interp_state_bind.
+      apply eq_itree_clo_bind with (UU := Logic.eq).
+      reflexivity.
+      intros [] [] EQ; inv EQ; reflexivity.
+    Qed.
+
+    Lemma interp_global_ret :
+      forall (R : Type) g (x: R),
+        runState (interp_global (Ret x: itree Effin R)) g ≅ Ret (g,x).
+    Proof.
+      intros; apply interp_state_ret.
+    Qed.
+
   End PARAMS.
 
 End Globals.
