src/coq/Handlers/UndefinedBehaviour.v
@@ -16,19 +16,19 @@ Set Contextual Implicit.
 Import MonadNotation.
 Open Scope monad_scope.
 
-Definition UB_handler {E}: UBE ~> PropT (itree E) := fun _ _ _ => True.
+Definition UB_handler {E}: UBE ~> PropT E := fun _ _ _ => True.
 
 Section PARAMS.
   Variable (E F: Type -> Type).
 
-  Definition E_trigger_prop : E ~> PropT (itree (E +' F)) :=
+  Definition E_trigger_prop : E ~> PropT (E +' F) :=
     fun R e => fun t => t = r <- trigger e ;; ret r.
 
-  Definition F_trigger_prop : F ~> PropT (itree (E +' F)) :=
+  Definition F_trigger_prop : F ~> PropT (E +' F) :=
     fun R e => fun t => t = r <- trigger e ;; ret r.
 
   Definition model_UB :
-    PropT (itree (E +' UBE +' F)) ~> PropT (itree (E +' F)) :=
+    PropT (E +' UBE +' F) ~> PropT (E +' F) :=
     fun T Pt t =>
       exists t', Pt t' /\ interp_prop (case_ E_trigger_prop (case_ UB_handler F_trigger_prop)) _ t' t.
 
